Day 1

problems/1/Problem1.dfy
@@ -1,15 +1,57 @@
 include "../../parser/split.dfy"
 include "../../parser/parseInt.dfy"
 module Problem1 {
-    import Std.Collections.Seq
+    import opened Split
+    import opened ParseInt
+    import opened Std.Collections.Seq
+    import opened Std.Relations
+
+    function abs(x: int): int {
+        if x < 0 then -x else x
+    }
+
+    method parseInput(input: string) returns (left: seq<int>, right: seq<int>) 
+        ensures |left| == |right|
+    {
+        left := [];
+        right := [];
+        var ids := splitOnBreak(input);
+        for i := 0 to |ids| 
+            invariant |left| == |right|
+        {
+            if ids[i] != "" {
+                var idsPieces := split(ids[i], "   ");
+                expect |idsPieces| == 2;
+                assume {:axiom} |idsPieces| == 2;
+                left := left+[Integer(idsPieces[0])];
+                right := right+[Integer(idsPieces[1])];
+            }
+        }
+    }
+
+    predicate lte(x: int, y: int) {
+        x <= y
+    }
+
+    function MapLists(left: seq<int>, right: seq<int>): seq<int> 
+        requires |left| == |right|
+    {
+        if |left| == 0 then [] else [abs(right[0]-left[0])]+MapLists(left[1..], right[1..])
+    }
 
     method problem1_1(input: string) returns (x: int)
     {
-        return 1;
+        var left, right := parseInput(input);
+        left := MergeSortBy(lte, left);
+        right := MergeSortBy(lte, right);
+        return FoldLeft((sum, val) => sum + val, 0, MapLists(left, right));
     }
 
     method problem1_2(input: string) returns (x: int)
     {
-        return 2;
+        var left, right := parseInput(input);
+        left := MergeSortBy(lte, left);
+        var rightms := multiset(right);
+        return  FoldLeft((sum, val) => sum + val, 0, Map((val:int) => val * rightms[val], left));
     }
 }
